Ethereum/Theory/ProgressLemmas.lean
@@ -2,6 +2,8 @@ import Ethereum.Semantics
 import Ethereum.UInt256
 import Ethereum.Data.Stack
 
+import Ethereum.Theory.NoOutOfFuel
+
 namespace Ethereum
 
 namespace EVM
@@ -41,14 +43,14 @@ lemma Xstep_X_X_continue : ∀ f state istate validJumps xres,
     rw [Xstep_env_unchanged state istate validJumps .none hstep0]
 
 lemma Xstep_X_X_halt_success : ∀ f state state' validJumps o,
-  Xstep validJumps state = .ok (state', .some (true, o))
+  Xstep validJumps state = .ok (state', .some (HaltCause.success, o))
   → X (f + 1) validJumps state = .ok (.success state' o) := by
     intros f state state' validJumps o hstep
     unfold X
     simp [hstep, bind, Except.bind]
 
 lemma Xstep_X_X_halt_revert : ∀ f state state' validJumps o,
-  Xstep validJumps state = .ok (state', .some (false,o))
+  Xstep validJumps state = .ok (state', .some (HaltCause.revert,o))
   → X (f + 1) validJumps state = .ok (.revert state'.machineState.gasAvailable o) := by
     intros f state state' validJumps o hstep
     unfold X
@@ -60,4 +62,90 @@ lemma Xstep_X_X_except : ∀ f state validJumps e,
     intros f state validJumps e hstep
     unfold X
     simp [hstep, bind, Except.bind]
+
+-- inductive Xstep_rel validJumps :  State → Except ExecutionException (State × Option (HaltCause × ByteArray)) → Prop where
+--   | intro {s} :
+--     Xstep_rel validJumps s (Xstep validJumps s)
+
+  
+inductive XstepN validJumps : State → Except ExecutionException (State × Option (HaltCause × ByteArray)) → ℕ → Prop where
+  | step : ∀ s s',
+    -- Xstep_rel validJumps s s' →
+    Xstep validJumps s = s' →
+    XstepN validJumps s s' 1
+  | trans : ∀ s s' x' n,
+    -- Xstep_rel validJumps s (.ok (s', .none)) →
+    Xstep validJumps s = .ok (s', .none) →
+    XstepN validJumps s' x' n →
+    XstepN validJumps s x' (n + 1)
+
+lemma XstepN_X_continue {s s' n f xres} validJumps :
+    XstepN validJumps s (.ok (s', .none)) n →
+    X f validJumps s' = xres →
+    X (f + n) validJumps s = xres := by
+    intro hstepN hX
+    generalize hxi : (Except.ok (s', none)) = xi
+    rw [hxi] at hstepN
+    induction hstepN with
+    | step s is hstep =>
+      rw [← hxi] at hstep
+      exact Xstep_X_X_continue f s s' validJumps xres hstep hX
+    | trans s s' x' n hstep hnsucc ih =>
+      unfold X  
+      simp [bind, Except.bind, hstep]
+      apply ih at hxi
+      simp [← hxi]
+      rw [Xstep_env_unchanged s s' validJumps .none hstep]
+
+lemma XstepN_X_halt_success {s s' o n f} validJumps :
+    XstepN validJumps s (.ok (s', .some (.success, o))) n →
+    X (f + n) validJumps s = .ok (.success s' o) := by
+    intro hstepN
+    generalize hxi : (Except.ok (s', Option.some (HaltCause.success, o))) = xi
+    rw [hxi] at hstepN
+    induction hstepN with
+    | step s is hstep =>
+      rw [← hxi] at hstep
+      exact Xstep_X_X_halt_success f s s' validJumps o hstep
+    | trans s s' x' n hstep hnsucc ih =>
+      unfold X  
+      simp [bind, Except.bind, hstep]
+      apply ih at hxi
+      simp [← hxi]
+      rw [Xstep_env_unchanged s s' validJumps .none hstep]
+
+lemma XstepN_X_halt_revert {s s' o n f} validJumps :
+    XstepN validJumps s (.ok (s', .some (.revert, o))) n →
+    X (f + n) validJumps s = .ok (.revert s'.machineState.gasAvailable o) := by
+    intro hstepN
+    generalize hxi : (Except.ok (s', Option.some (HaltCause.revert, o))) = xi
+    rw [hxi] at hstepN
+    induction hstepN with
+    | step s is hstep =>
+      rw [← hxi] at hstep
+      exact Xstep_X_X_halt_revert f s s' validJumps o hstep
+    | trans s s' x' n hstep hnsucc ih =>
+      unfold X  
+      simp [bind, Except.bind, hstep]
+      apply ih at hxi
+      simp [← hxi]
+      rw [Xstep_env_unchanged s s' validJumps .none hstep]
+
+lemma XstepN_XstepN_add { s s' n x m} validJumps :
+    XstepN validJumps s (.ok (s', .none)) n →
+    XstepN validJumps s' x m →
+    XstepN validJumps s x (n + m) := by
+  intro hstepn hstepm
+  generalize hxi : (Except.ok (s', none)) = xi
+  rw [hxi] at hstepn
+  induction hstepn with
+  | step s is hstep =>
+    rw [← hxi] at hstep
+    rw [Nat.add_comm]
+    exact XstepN.trans s s' x m hstep hstepm
+  | trans s is x' n hstep hnsucc ih =>
+    apply ih at hxi
+    rw [Nat.add_comm]
+    rw [Nat.add_comm] at hxi
+    exact XstepN.trans s is x (m + n) hstep hxi
 
