Ethereum/Theory/NoOutOfFuel.lean
@@ -1,0 +1,344 @@
+import Ethereum.Semantics
+import Ethereum.UInt256
+import Ethereum.Data.Stack
+
+namespace Ethereum
+
+namespace EVM
+
+set_option maxHeartbeats 2000000 in
+lemma Z_no_OutOfFuel {w s} validJumps :
+  -- Z validJumps w s = .error e → e ≠ .OutOfFuel := by
+  Z validJumps w s ≠ .error .OutOfFuel := by
+    intro h
+    simp [Z] at h
+    cases hd : δ w
+    · simp [hd] at h
+    · simp [hd] at h
+      rename_i val
+      by_cases hd' : List.length s.machineState.stack < val
+      · simp [hd'] at h
+      · simp [hd'] at h
+        repeat (split at h <;> try simp at h)
+
+@[simp] private lemma execUnOp_no_OutOfFuel (f : Primop.Unary) (s : State) :
+    execUnOp f s ≠ .error .OutOfFuel := by
+  unfold execUnOp
+  split <;> simp
+
+@[simp] private lemma execBinOp_no_OutOfFuel (f : Primop.Binary) (s : State) :
+    execBinOp f s ≠ .error .OutOfFuel := by
+  unfold execBinOp
+  split <;> simp
+
+@[simp] private lemma execTriOp_no_OutOfFuel (f : Primop.Ternary) (s : State) :
+    execTriOp f s ≠ .error .OutOfFuel := by
+  unfold execTriOp
+  split <;> simp
+
+@[simp] private lemma executionEnvOp_no_OutOfFuel (op : ExecutionEnv → UInt256) (s : State) :
+    executionEnvOp op s ≠ .error .OutOfFuel := by
+  unfold executionEnvOp
+  simp
+
+@[simp] private lemma unaryExecutionEnvOp_no_OutOfFuel
+    (op : ExecutionEnv → UInt256 → UInt256) (s : State) :
+    unaryExecutionEnvOp op s ≠ .error .OutOfFuel := by
+  unfold unaryExecutionEnvOp
+  split <;> simp
+
+@[simp] private lemma machineStateOp_no_OutOfFuel (op : MachineState → UInt256) (s : State) :
+    machineStateOp op s ≠ .error .OutOfFuel := by
+  unfold machineStateOp
+  simp
+
+@[simp] private lemma binaryMachineStateOp_no_OutOfFuel
+    (op : MachineState → UInt256 → UInt256 → MachineState) (s : State) :
+    binaryMachineStateOp op s ≠ .error .OutOfFuel := by
+  unfold binaryMachineStateOp
+  split <;> simp
+
+@[simp] private lemma binaryMachineStateOp'_no_OutOfFuel
+    (op : MachineState → UInt256 → UInt256 → UInt256 × MachineState) (s : State) :
+    binaryMachineStateOp' op s ≠ .error .OutOfFuel := by
+  unfold binaryMachineStateOp'
+  split <;> simp
+
+@[simp] private lemma ternaryMachineStateOp_no_OutOfFuel
+    (op : MachineState → UInt256 → UInt256 → UInt256 → MachineState) (s : State) :
+    ternaryMachineStateOp op s ≠ .error .OutOfFuel := by
+  unfold ternaryMachineStateOp
+  split <;> simp
+
+@[simp] private lemma binaryStateOp_no_OutOfFuel
+    (op : State → UInt256 → UInt256 → State) (s : State) :
+    binaryStateOp op s ≠ .error .OutOfFuel := by
+  unfold binaryStateOp
+  split <;> simp
+
+@[simp] private lemma stateOp_no_OutOfFuel (op : State → UInt256) (s : State) :
+    stateOp op s ≠ .error .OutOfFuel := by
+  unfold stateOp
+  simp
+
+@[simp] private lemma unaryStateOp_no_OutOfFuel
+    (op : State → UInt256 → State × UInt256) (s : State) :
+    unaryStateOp op s ≠ .error .OutOfFuel := by
+  unfold unaryStateOp
+  split <;> simp
+
+@[simp] private lemma ternaryCopyOp_no_OutOfFuel
+    (op : State → UInt256 → UInt256 → UInt256 → State) (s : State) :
+    ternaryCopyOp op s ≠ .error .OutOfFuel := by
+  unfold ternaryCopyOp
+  split <;> simp
+
+@[simp] private lemma quaternaryCopyOp_no_OutOfFuel
+    (op : State → UInt256 → UInt256 → UInt256 → UInt256 → State) (s : State) :
+    quaternaryCopyOp op s ≠ .error .OutOfFuel := by
+  unfold quaternaryCopyOp
+  split <;> simp
+
+@[simp] private lemma log0Op_no_OutOfFuel (s : State) :
+    log0Op s ≠ .error .OutOfFuel := by
+  unfold log0Op
+  split <;> simp
+
+@[simp] private lemma log1Op_no_OutOfFuel (s : State) :
+    log1Op s ≠ .error .OutOfFuel := by
+  unfold log1Op
+  split <;> simp
+
+@[simp] private lemma log2Op_no_OutOfFuel (s : State) :
+    log2Op s ≠ .error .OutOfFuel := by
+  unfold log2Op
+  split <;> simp
+
+@[simp] private lemma log3Op_no_OutOfFuel (s : State) :
+    log3Op s ≠ .error .OutOfFuel := by
+  unfold log3Op
+  split <;> simp
+
+@[simp] private lemma log4Op_no_OutOfFuel (s : State) :
+    log4Op s ≠ .error .OutOfFuel := by
+  unfold log4Op
+  split <;> simp
+
+@[simp] private lemma dup_no_OutOfFuel (n : ℕ) (s : State) :
+    dup n s ≠ .error .OutOfFuel := by
+  simp [dup]
+  by_cases h : n ≤ s.machineState.stack.length <;> simp [h]
+
+@[simp] private lemma swap_no_OutOfFuel (n : ℕ) (s : State) :
+    swap n s ≠ .error .OutOfFuel := by
+  simp [swap]
+  by_cases h : n + 1 ≤ s.machineState.stack.length <;> simp [h]
+
+@[simp] private lemma call_ne_error
+    (gasCost : Nat)
+    (blobVersionedHashes : List ByteArray)
+    (gas source recipient t value value' inOffset inSize outOffset outSize : UInt256)
+    (permission : Bool)
+    (evmState : State)
+    (e : ExecutionException) :
+    call gasCost blobVersionedHashes gas source recipient t value value' inOffset inSize
+        outOffset outSize permission evmState ≠ .error e := by
+  unfold call
+  simp
+
+set_option maxHeartbeats 2000000 in
+private lemma step_create_no_OutOfFuel {g state arg} :
+    step g (.CREATE, arg) state ≠ .error .OutOfFuel := by
+  intro hstep
+  unfold step at hstep
+  simp [bind, Except.bind] at hstep
+  split at hstep
+  · split at hstep
+    · split at hstep
+      · simp at hstep
+      · split at hstep
+        · rename_i heq
+          simp [pure, Except.pure] at heq
+        · simp at hstep
+    · split at hstep
+      · split at hstep
+        · simp at hstep
+        · split at hstep
+          · rename_i heq
+            simp [pure, Except.pure] at heq
+          · split at hstep
+            · split at hstep <;> simp at hstep
+            · simp at hstep
+      · split at hstep
+        · simp at hstep
+        · split at hstep
+          · rename_i heq
+            simp [pure, Except.pure] at heq
+          · split at hstep
+            · split at hstep <;> simp at hstep
+            · simp at hstep
+  · simp at hstep
+
+set_option maxHeartbeats 2000000 in
+private lemma step_create2_no_OutOfFuel {g state arg} :
+    step g (.CREATE2, arg) state ≠ .error .OutOfFuel := by
+  intro hstep
+  unfold step at hstep
+  simp [bind, Except.bind] at hstep
+  split at hstep
+  · split at hstep
+    · split at hstep
+      · simp at hstep
+      · split at hstep
+        · rename_i heq
+          simp [pure, Except.pure] at heq
+        · simp at hstep
+    · split at hstep
+      · split at hstep
+        · simp at hstep
+        · split at hstep
+          · rename_i heq
+            simp [pure, Except.pure] at heq
+          · split at hstep
+            · split at hstep <;> simp at hstep
+            · simp at hstep
+      · split at hstep
+        · simp at hstep
+        · split at hstep
+          · rename_i heq
+            simp [pure, Except.pure] at heq
+          · split at hstep
+            · split at hstep <;> simp at hstep
+            · simp at hstep
+  · simp at hstep
+
+private lemma step_call_no_OutOfFuel {g state arg} :
+    step g (.CALL, arg) state ≠ .error .OutOfFuel := by
+  intro h
+  simp [step, bind, Except.bind, liftM, monadLift, MonadLift.monadLift] at h
+  cases hpop : state.machineState.stack.pop7 <;> simp [hpop, Option.option] at h
+  split at h <;> simp at *
+
+private lemma step_callcode_no_OutOfFuel {g state arg} :
+    step g (.CALLCODE, arg) state ≠ .error .OutOfFuel := by
+  intro h
+  simp [step, bind, Except.bind, liftM, monadLift, MonadLift.monadLift] at h
+  cases hpop : state.machineState.stack.pop7 <;> simp [hpop, Option.option] at h
+  split at h <;> simp at *
+
+private lemma step_delegatecall_no_OutOfFuel {g state arg} :
+    step g (.DELEGATECALL, arg) state ≠ .error .OutOfFuel := by
+  intro h
+  simp [step, bind, Except.bind, liftM, monadLift, MonadLift.monadLift] at h
+  cases hpop : state.machineState.stack.pop6 <;> simp [hpop, Option.option] at h
+  split at h <;> simp at *
+
+private lemma step_staticcall_no_OutOfFuel {g state arg} :
+    step g (.STATICCALL, arg) state ≠ .error .OutOfFuel := by
+  intro h
+  simp [step, bind, Except.bind, liftM, monadLift, MonadLift.monadLift] at h
+  cases hpop : state.machineState.stack.pop6 <;> simp [hpop, Option.option] at h
+  split at h <;> simp at *
+
+private lemma step_selfdestruct_no_OutOfFuel {g state arg} :
+    step g (.SELFDESTRUCT, arg) state ≠ .error .OutOfFuel := by
+  intro h
+  simp [step] at h
+  cases hpop : state.machineState.stack.pop <;> simp [hpop] at h
+  repeat (split at h <;> simp at h)
+
+set_option maxHeartbeats 2000000 in
+lemma step_no_OutOfFuel {g state} instr :
+  step g instr state ≠ .error .OutOfFuel := by
+  rcases instr with ⟨instr, arg⟩
+  cases instr with
+  | StopArith op =>
+      cases op <;> intro h <;> simp [step] at h
+  | CompBit op =>
+      cases op <;> intro h <;> simp [step] at h
+  | Keccak op =>
+      cases op
+      intro h
+      simp [step] at h
+  | Env op =>
+      cases op <;> intro h <;>
+        simp [step] at h <;>
+        repeat (split at h) <;>
+        simp at h
+  | Block op =>
+      cases op <;> intro h <;> simp [step] at h
+  | StackMemFlow op =>
+      cases op <;> intro h <;>
+        simp [step] at h <;>
+        repeat (split at h) <;>
+        simp at h
+  | Push op =>
+      cases op <;> intro h <;>
+        simp [step] at h <;>
+        repeat (split at h) <;>
+        simp at h
+  | Dup op =>
+      cases op <;> intro h <;> simp [step] at h
+  | Exchange op =>
+      cases op <;> intro h <;> simp [step] at h
+  | Log op =>
+      cases op <;> intro h <;> simp [step] at h
+  | System op =>
+      cases op
+      · exact step_create_no_OutOfFuel
+      · exact step_call_no_OutOfFuel
+      · exact step_callcode_no_OutOfFuel
+      · intro h
+        simp [step] at h
+      · exact step_delegatecall_no_OutOfFuel
+      · exact step_create2_no_OutOfFuel
+      · exact step_staticcall_no_OutOfFuel
+      · intro h
+        simp [step] at h
+      · intro h
+        simp [step] at h
+      · exact step_selfdestruct_no_OutOfFuel
+
+
+lemma Xstep_no_OutOfFuel {state} validJumps :
+  Xstep validJumps state ≠ .error .OutOfFuel := by
+    simp [Xstep]
+    intro hstep
+    split at hstep
+    · rename_i heq; simp at hstep; rw [hstep] at heq; simp [Z_no_OutOfFuel] at heq
+    · split at hstep <;>
+      · simp [bind, Except.bind] at hstep
+        split at hstep
+        · rename_i heq; simp at hstep; simp [hstep] at heq
+          apply step_no_OutOfFuel; exact heq
+        · repeat (split at hstep <;> try simp at hstep)
+
+lemma Xstep_of_gas_reduce_gt_1 {state state' o} validJumps :
+  Xstep validJumps state = .ok (state', o) →
+  state.machineState.gasAvailable.toNat - state'.machineState.gasAvailable.toNat > 1 := by sorry
+
+lemma X_no_OufOfFuel_of_gas_lt_fuel {f s} validJumps : 
+  s.machineState.gasAvailable.toNat < f →
+  X f validJumps s ≠ .error .OutOfFuel := by
+  intro h
+  revert s
+  induction f with
+  | zero => intro s h; simp at h
+  | succ f' ih =>
+    intro s h
+    unfold X
+    simp [bind, Except.bind]
+    split
+    · rename_i hstep;
+      simp
+      have h' : Xstep validJumps s ≠ .error .OutOfFuel := Xstep_no_OutOfFuel validJumps
+      simp [hstep] at h'
+      assumption
+    · rename_i is hstep
+      split
+      · apply ih
+        · simp
+          apply Xstep_of_gas_reduce_gt_1 at hstep
+          omega
+      · simp
+      · simp
